modules/testgen/src/main/scala/specrest/testgen/Stateful.scala
@@ -835,7 +835,7 @@ object Stateful:
         |$statefulImportLine
         |)
         |
-        |from tests.conftest import client
+        |from tests.conftest import client, request_without_redirects
         |from tests.predicates import is_valid_email, is_valid_uri
         |from tests.redaction import redact
         |
