modules/parser/src/main/resources/specrest/parser/preamble.spec
@@ -1,6 +1,6 @@
 service Preamble {
 
-  predicate isValidURI(s: String) = s matches /^https?:..[^\s]+/
+  predicate isValidURI(s: String) = s matches /^https?:\/\/[^\s]+/
 
   predicate isValidEmail(s: String) = s matches /^[^@\s]+@[^@\s]+\.[^@\s]+$/
 
